@prefix envthes: <http://vocabs.lter-europe.net/EnvThes/> .
@prefix skos: <http://www.w3.org/2004/02/skos/core#> .
@prefix iadopt: <https://w3id.org/iadopt/ont/> .
@prefix rdfs: <http://www.w3.org/2000/01/rdf-schema#> .
@prefix owl: <http://www.w3.org/2002/07/owl#> .
@prefix dc: <http://purl.org/dc/terms/> .
@prefix xsd: <http://www.w3.org/2001/XMLSchema#> .

envthes:20935
  skos:prefLabel "variable"@en ;
  a skos:Concept ;
  skos:narrower envthes:30382 .

iadopt:Variable
  rdfs:label "Variable" ;
  a owl:Class .

iadopt:hasProperty
  rdfs:comment "A Variable has a Property that characterizes an Entity." ;
  rdfs:label "hasProperty" .

envthes:30382
  dc:created "2024-10-14"^^xsd:date ;
  iadopt:hasContextObject <https://terra-vocabulary.org/ncl/FAIR-Incubator/earthfeaturetype/c_07d7a262> ;
  skos:altLabel "maximum acceleration of ground during seismic events"@en ;
  skos:broader envthes:20935 ;
  dc:modified "2024-10-14"^^xsd:date ;
  iadopt:hasObjectOfInterest envthes:30365 ;
  a skos:Concept, iadopt:Variable ;
  skos:prefLabel "peak ground acceleration during seismic events"@en ;
  skos:inScheme envthes: ;
  iadopt:hasProperty <https://qudt.org/vocab/quantitykind/Acceleration> ;
  skos:definition "Maximum acceleration measured on the earth surface during seismic events (e.g., earthquakes.)"@en ;
  iadopt:hasMatrix <http://purl.obolibrary.org/obo/RBO_00000017> .

iadopt:hasMatrix
  rdfs:subPropertyOf iadopt:hasContextObject ;
  rdfs:comment "A Variable might have an Entity in which the ObjectOfInterest is contained." ;
  rdfs:label "hasMatrix" .

envthes:
  skos:prefLabel "EnvThes"@en ;
  a owl:Ontology, skos:ConceptScheme .

envthes:30365
  skos:prefLabel "ground"@en ;
  a skos:Concept .

iadopt:hasObjectOfInterest
  rdfs:comment "A Variable has an Entity whose Property is observed." ;
  rdfs:label "hasObjectOfInterest" .

iadopt:hasContextObject
  rdfs:comment "A Variable has an Entity that provides additional background information regarding the ObjectOfInterest." ;
  rdfs:label "hasContextObject" .
