@prefix envthes: <http://vocabs.lter-europe.net/EnvThes/> .
@prefix skos: <http://www.w3.org/2004/02/skos/core#> .
@prefix iadopt: <https://w3id.org/iadopt/ont/> .
@prefix rdfs: <http://www.w3.org/2000/01/rdf-schema#> .
@prefix owl: <http://www.w3.org/2002/07/owl#> .
@prefix elter_cl: <http://vocabs.lter-europe.net/elter_cl/> .
@prefix dc: <http://purl.org/dc/terms/> .
@prefix xsd: <http://www.w3.org/2001/XMLSchema#> .

envthes:20935
  skos:prefLabel "variable"@en ;
  a skos:Concept ;
  skos:narrower envthes:30400 .

iadopt:Variable
  rdfs:label "Variable" ;
  a owl:Class .

iadopt:hasProperty
  rdfs:comment "A Variable has a Property that characterizes an Entity." ;
  rdfs:label "hasProperty" .

envthes:
  skos:prefLabel "EnvThes"@en ;
  a owl:Ontology, skos:ConceptScheme .

iadopt:hasObjectOfInterest
  rdfs:comment "A Variable has an Entity whose Property is observed." ;
  rdfs:label "hasObjectOfInterest" .

envthes:30400
  a skos:Concept, iadopt:Variable ;
  iadopt:hasContextObject <http://purl.bioontology.org/ontology/LNC/LP73352-4> ;
  skos:inScheme envthes: ;
  skos:prefLabel "distance to nearest neighbour EUNIS habitat patch"@en ;
  skos:broader envthes:20935 ;
  iadopt:hasProperty <https://qudt.org/vocab/quantitykind/Distance> ;
  iadopt:hasConstraint elter_cl:10597, envthes:30401 ;
  dc:created "2024-10-31"^^xsd:date ;
  dc:creator <https://orcid.org/0000-0003-2195-3997> ;
  dc:modified "2024-10-31"^^xsd:date ;
  iadopt:hasObjectOfInterest envthes:21894 ;
  skos:definition "The distance to the nearest neighbour is a metric used to measure the degree of connection of EUNIS habitats within a landscape, in terms of their spatial distribution."@en .

iadopt:hasContextObject
  rdfs:comment "A Variable has an Entity that provides additional background information regarding the ObjectOfInterest." ;
  rdfs:label "hasContextObject" .

iadopt:hasConstraint
  rdfs:comment "A Variable has a Constraint, that confines an Entity involved in the observation." ;
  rdfs:label "hasConstraint" .

envthes:21894
  skos:prefLabel "habitat"@en ;
  a skos:Concept .

<http://purl.bioontology.org/ontology/LNC/LP73352-4>
rdfs:label "site".

envthes:30401
  skos:prefLabel "nearest neighbour"@en ;
  a iadopt:Constraint, skos:Concept ;
  iadopt:constrains envthes:21894 .

<http://vocabs.lter-europe.net/elter_cl/10597>
  skos:prefLabel "EUNIS"@en ;
  a iadopt:Constraint, skos:Concept ;
  iadopt:constrains envthes:21894 .
