@prefix envthes: <http://vocabs.lter-europe.net/EnvThes/> .
@prefix skos: <http://www.w3.org/2004/02/skos/core#> .
@prefix dc: <http://purl.org/dc/terms/> .
@prefix xsd: <http://www.w3.org/2001/XMLSchema#> .
@prefix iadopt: <https://w3id.org/iadopt/ont/> .
@prefix rdfs: <http://www.w3.org/2000/01/rdf-schema#> .
@prefix owl: <http://www.w3.org/2002/07/owl#> .

envthes:20935
  skos:prefLabel "variable"@en ;
  a skos:Concept ;
  skos:narrower envthes:30404 .

envthes:30404
  dc:created "2024-10-31"^^xsd:date ;
  iadopt:hasMatrix <http://purl.obolibrary.org/obo/GSSO_005261> ;
  iadopt:hasObjectOfInterest <http://purl.bioontology.org/ontology/npo#NPO_199> ;
  iadopt:hasProperty <https://qudt.org/vocab/quantitykind/ParticleFluence> ;
  skos:broader envthes:20935 ;
  a iadopt:Variable, skos:Concept ;
  skos:definition "Particle number of nanomaterial internalised by a specific cell area and and time."@en ;
  skos:inScheme envthes: ;
  dc:creator <https://orcid.org/0000-0003-2195-3997> ;
  iadopt:hasConstraint envthes:21952 ;
  dc:modified "2024-10-31"^^xsd:date ;
  skos:prefLabel "dose (number) of applied nanomaterial internalised by a specific cell population"@en .

iadopt:Variable
  rdfs:label "Variable" ;
  a owl:Class .

iadopt:hasProperty
  rdfs:comment "A Variable has a Property that characterizes an Entity." ;
  rdfs:label "hasProperty" .

iadopt:hasMatrix
  rdfs:subPropertyOf iadopt:hasContextObject ;
  rdfs:comment "A Variable might have an Entity in which the ObjectOfInterest is contained." ;
  rdfs:label "hasMatrix" .

envthes:
  skos:prefLabel "EnvThes"@en ;
  a owl:Ontology, skos:ConceptScheme .

envthes:21952
  skos:prefLabel "absorbed"@en ;
  a iadopt:Constraint, skos:Concept ;
  iadopt:constrains <http://purl.bioontology.org/ontology/npo#NPO_199> .

iadopt:hasObjectOfInterest
  rdfs:comment "A Variable has an Entity whose Property is observed." ;
  rdfs:label "hasObjectOfInterest" .

iadopt:hasConstraint
  rdfs:comment "A Variable has a Constraint, that confines an Entity involved in the observation." ;
  rdfs:label "hasConstraint" .
