@prefix envthes: <http://vocabs.lter-europe.net/EnvThes/> .
@prefix skos: <http://www.w3.org/2004/02/skos/core#> .
@prefix iadopt: <https://w3id.org/iadopt/ont/> .
@prefix rdfs: <http://www.w3.org/2000/01/rdf-schema#> .
@prefix owl: <http://www.w3.org/2002/07/owl#> .
@prefix dc: <http://purl.org/dc/terms/> .
@prefix xsd: <http://www.w3.org/2001/XMLSchema#> .

envthes:20935
  skos:prefLabel "variable"@en ;
  a skos:Concept ;
  skos:narrower envthes:30385 .

iadopt:Variable
  rdfs:label "Variable" ;
  a owl:Class .

iadopt:hasProperty
  rdfs:comment "A Variable has a Property that characterizes an Entity." ;
  rdfs:label "hasProperty" .

envthes:20905
  skos:prefLabel "surface sediment"@en ;
  a skos:Concept .

iadopt:hasMatrix
  rdfs:subPropertyOf iadopt:hasContextObject ;
  rdfs:comment "A Variable might have an Entity in which the ObjectOfInterest is contained." ;
  rdfs:label "hasMatrix" .

envthes:
  skos:prefLabel "EnvThes"@en ;
  a owl:Ontology, skos:ConceptScheme .

iadopt:hasObjectOfInterest
  rdfs:comment "A Variable has an Entity whose Property is observed." ;
  rdfs:label "hasObjectOfInterest" .

<http://purl.obolibrary.org/obo/ENVO_01000063>
  skos:prefLabel "planctonic material"@en ;
  a iadopt:Constraint, skos:Concept ;
  iadopt:constrains <https://www.gbif.org/species/8376456> .

envthes:30385
  skos:altLabel "size of planktic foraminifers in surface sediments"@en ;
  skos:inScheme envthes: ;
  a skos:Concept, iadopt:Variable ;
  dc:modified "2024-10-14"^^xsd:date ;
  skos:broader envthes:20935 ;
  iadopt:hasProperty <https://qudt.org/vocab/quantitykind/Diameter> ;
  iadopt:hasMatrix envthes:20905 ;
  skos:definition "Mean_size of planktic foraminifers in surface sediments. Size is defined as mean diameter in the plane of largest extent, and mean size is defined as the arithmetic average of a population (i.e., a sample of specimen)."@en ;
  iadopt:hasConstraint <http://purl.obolibrary.org/obo/ENVO_01000063> ;
  iadopt:hasObjectOfInterest <https://www.gbif.org/species/8376456> ;
  skos:prefLabel "planctic Foraminifera size in surface sediments"@en ;
  dc:created "2024-10-14"^^xsd:date .

iadopt:hasConstraint
  rdfs:comment "A Variable has a Constraint, that confines an Entity involved in the observation." ;
  rdfs:label "hasConstraint" .
