@prefix envthes: <http://vocabs.lter-europe.net/EnvThes/> .
@prefix skos: <http://www.w3.org/2004/02/skos/core#> .
@prefix iadopt: <https://w3id.org/iadopt/ont/> .
@prefix rdfs: <http://www.w3.org/2000/01/rdf-schema#> .
@prefix owl: <http://www.w3.org/2002/07/owl#> .
@prefix dc: <http://purl.org/dc/terms/> .
@prefix xsd: <http://www.w3.org/2001/XMLSchema#> .

envthes:20935
  skos:prefLabel "variable"@en ;
  a skos:Concept ;
  skos:narrower envthes:30396 .

iadopt:Variable
  rdfs:label "Variable" ;
  a owl:Class .

iadopt:hasProperty
  rdfs:comment "A Variable has a Property that characterizes an Entity." ;
  rdfs:label "hasProperty" .

iadopt:hasMatrix
  rdfs:subPropertyOf iadopt:hasContextObject ;
  rdfs:comment "A Variable might have an Entity in which the ObjectOfInterest is contained." ;
  rdfs:label "hasMatrix" .

envthes:
  skos:prefLabel "EnvThes"@en ;
  a owl:Ontology, skos:ConceptScheme .

envthes:21994
  skos:prefLabel "minimum"@en ;
  a iadopt:Constraint, skos:Concept ;
  iadopt:constrains envthes:21543 .

iadopt:hasObjectOfInterest
  rdfs:comment "A Variable has an Entity whose Property is observed." ;
  rdfs:label "hasObjectOfInterest" .

envthes:30396
  a skos:Concept, iadopt:Variable ;
  dc:creator <https://orcid.org/0000-0003-2195-3997> ;
  iadopt:hasConstraint envthes:21994 ;
  skos:inScheme envthes: ;
  skos:prefLabel "height of atmospheric boundary layer"@en ;
  iadopt:hasObjectOfInterest envthes:21543 ;
  dc:created "2024-10-31"^^xsd:date ;
  skos:broader envthes:20935 ;
  skos:definition "The depth of the lowest layer of the atmosphere measured above the surface of the ground."@en ;
  iadopt:hasMatrix <http://purl.obolibrary.org/obo/ENVO_01000540> ;
  dc:modified "2024-10-31"^^xsd:date ;
  iadopt:hasProperty <http://www.ontology-of-units-of-measure.org/resource/om-2/Height> .

iadopt:hasConstraint
  rdfs:comment "A Variable has a Constraint, that confines an Entity involved in the observation." ;
  rdfs:label "hasConstraint" .

envthes:21543
  skos:prefLabel "atmospheric boundary layer"@en ;
  a skos:Concept .
